Allow more fine-grained specification of exception case
... when proving the CHERI properties:  Add a parameter to specify which
types of (Sail) exceptions signal an ISA exception, and don't consider
internal failures to signal an exception any more.  Also add the option
to thread through well-formedness assumptions (e.g. that register reads
are well-typed) that help rule out internal failures.

model/Recognising_Automata.thy
@@ -601,7 +601,7 @@ lemma non_cap_exp_throw[non_cap_expI]:
   "non_cap_exp (throw e)"
   by (auto simp: non_cap_exp_def)
 
-lemma non_cap_exp_early_return[non_cap_expI]:
+lemma non_cap_exp_early_return[intro!]:
   "non_cap_exp (early_return a)"
   by (auto simp: early_return_def intro!: non_cap_expI)
 
@@ -620,6 +620,10 @@ lemma non_cap_exp_liftR[intro!]:
 lemma non_mem_exp_liftR:
   "non_mem_exp (liftR m)" if "non_mem_exp m"
   by (auto simp: liftR_def intro!: that non_mem_exp_try_catch non_cap_expI[THEN non_cap_exp_non_mem_exp])
+
+lemma non_mem_exp_early_return[intro!]:
+  "non_mem_exp (early_return a)"
+  by (auto simp: early_return_def intro!: non_cap_expI[THEN non_cap_exp_non_mem_exp])
 
 lemma non_cap_exp_assert_exp[non_cap_expI]:
   "non_cap_exp (assert_exp c msg)"
@@ -794,7 +798,8 @@ lemmas non_cap_exp_combinators =
 
 method non_cap_expI_base uses intro =
   (rule intro non_cap_expI non_cap_exp_split[THEN iffD2] non_cap_exp_combinators
-        non_cap_exp_read_non_cap_reg non_cap_exp_write_non_cap_reg allI impI conjI)+
+        non_cap_exp_read_non_cap_reg non_cap_exp_write_non_cap_reg non_cap_exp_early_return
+        allI impI conjI)+
 
 method non_cap_expI uses simp intro = (non_cap_expI_base intro: intro; simp add: simp)
 
@@ -813,7 +818,7 @@ lemmas non_mem_exp_combinators =
 
 method non_mem_expI uses simp intro =
   (intro intro non_mem_expI non_mem_exp_split[THEN iffD2] non_mem_exp_combinators
-         non_cap_expI[THEN non_cap_exp_non_mem_exp] allI impI conjI;
+         non_cap_expI[THEN non_cap_exp_non_mem_exp] non_mem_exp_early_return allI impI conjI;
    simp add: simp)
 
 lemma Run_write_reg_no_cap[trace_simp]:
@@ -1360,10 +1365,14 @@ locale Cap_Axiom_Assm_Automaton =
     and enabled :: "('cap, 'regval) axiom_state \<Rightarrow> 'regval event \<Rightarrow> bool"
     and use_mem_caps :: bool +
   fixes ex_traces :: bool
+    and is_isa_exception :: "'e \<Rightarrow> bool"
     and ev_assms :: "('cap, 'regval) axiom_state \<Rightarrow> 'regval event \<Rightarrow> bool"
+    and wellformed_ev :: "'regval event \<Rightarrow> bool"
   assumes non_cap_event_enabled: "\<And>e. non_cap_event e \<Longrightarrow> enabled s e"
     and read_non_special_regs_enabled: "\<And>r v. r \<notin> PCC ISA \<union> IDC ISA \<union> KCC ISA \<union> read_privileged_regs ISA \<Longrightarrow> enabled s (E_read_reg r v)"
 begin
+
+abbreviation "wellformed_trace t \<equiv> \<forall>e \<in> set t. wellformed_ev e"
 
 abbreviation "trace_assms \<equiv> holds_along_trace ev_assms"
 
@@ -1374,11 +1383,14 @@ definition accessed_caps_invariant :: "('cap, 'regval) axiom_state \<Rightarrow>
 definition accessed_caps_trace_invariant :: "('cap, 'regval) axiom_state \<Rightarrow> 'regval event list \<Rightarrow> bool" where
   "accessed_caps_trace_invariant s t \<equiv> (\<forall>i \<le> length t. accessed_caps_invariant (run s (take i t)))"
 
-definition pre_inv_trace_assms :: "('cap, 'regval) axiom_state \<Rightarrow> 'regval event list \<Rightarrow> bool" where
-  "pre_inv_trace_assms s t \<equiv> accessed_caps_trace_invariant s (butlast t) \<and> trace_assms s t"
+fun pre_inv_trace_assms :: "('cap, 'regval) axiom_state \<Rightarrow> nat \<Rightarrow> 'regval event list \<Rightarrow> bool" where
+  "pre_inv_trace_assms s (Suc n) (e # t) =
+     (accessed_caps_invariant s \<and> ev_assms s e \<and> wellformed_ev e \<and> pre_inv_trace_assms (axiom_step s e) n t)"
+| "pre_inv_trace_assms _ 0 t = wellformed_trace t"
+| "pre_inv_trace_assms _ _ _ = False"
 
 definition inv_trace_assms :: "('cap, 'regval) axiom_state \<Rightarrow> 'regval event list \<Rightarrow> bool" where
-  "inv_trace_assms s t \<equiv> accessed_caps_trace_invariant s t \<and> trace_assms s t"
+  "inv_trace_assms s t \<equiv> accessed_caps_trace_invariant s t \<and> trace_assms s t \<and> wellformed_trace t"
 
 lemma inv_trace_assms_trace_assms[simp, accessible_regsE, derivable_capsE]:
   assumes "inv_trace_assms s t"
@@ -1408,49 +1420,86 @@ lemma accessed_caps_trace_invariant_append_iff:
   "accessed_caps_trace_invariant s (t @ t') \<longleftrightarrow> accessed_caps_trace_invariant s t \<and> accessed_caps_trace_invariant (run s t) t'"
   by (induction t arbitrary: s) auto
 
-lemma pre_inv_trace_assms_Nil[simp]:
-  "pre_inv_trace_assms s [] \<longleftrightarrow> accessed_caps_invariant s"
-  by (auto simp: pre_inv_trace_assms_def accessed_caps_trace_invariant_def)
+lemma pre_inv_trace_assms_iff:
+  "pre_inv_trace_assms s n t \<longleftrightarrow>
+   (n \<le> length t \<and> (n > 0 \<longrightarrow> accessed_caps_trace_invariant s (take (n - 1) t)) \<and>
+    trace_assms s (take n t) \<and> wellformed_trace t)"
+  by (induction s n t rule: pre_inv_trace_assms.induct) (auto simp: take_Cons split: nat.split)
 
-lemma pre_inv_trace_assms_Cons:
-  "pre_inv_trace_assms s (e # t) \<longleftrightarrow>
-   accessed_caps_invariant s \<and> ev_assms s e \<and> (t = [] \<or> pre_inv_trace_assms (axiom_step s e) t)"
-  by (auto simp: pre_inv_trace_assms_def)
+lemma pre_inv_trace_assms_Nil[simp]:
+  "pre_inv_trace_assms s n [] \<longleftrightarrow> n = 0"
+  by (induction s n "[] :: 'regval trace" rule: pre_inv_trace_assms.induct) auto
+
+lemma pre_inv_trace_assms_accessed_caps_invariant_or_zero:
+  "pre_inv_trace_assms s n t \<Longrightarrow> n = 0 \<or> accessed_caps_invariant s"
+  by (elim pre_inv_trace_assms.elims) auto
+
+lemma pre_inv_trace_assms_accessed_caps_invariant:
+  "pre_inv_trace_assms s n t \<Longrightarrow> n > 0 \<Longrightarrow> accessed_caps_invariant s"
+  by (auto dest: pre_inv_trace_assms_accessed_caps_invariant_or_zero)
 
 lemma pre_inv_trace_assms_append_iff:
-  "pre_inv_trace_assms s (t @ t') \<longleftrightarrow>
-   pre_inv_trace_assms s t \<and> (t' = [] \<or> pre_inv_trace_assms (run s t) t' \<and> accessed_caps_invariant (run s t))"
-  by (induction t arbitrary: s; cases t'; fastforce simp: pre_inv_trace_assms_Cons)
+  "pre_inv_trace_assms s n (t @ t') \<longleftrightarrow>
+   (pre_inv_trace_assms s (min n (length t)) t \<and> pre_inv_trace_assms (run s t) (n - length t) t' \<and>
+    (n > length t \<longrightarrow> accessed_caps_invariant (run s t)))"
+  by (induction s n t rule: pre_inv_trace_assms.induct)
+     (auto intro: pre_inv_trace_assms_accessed_caps_invariant)
+
+lemma pre_inv_trace_assms_wellformed_trace:
+  "pre_inv_trace_assms s n t \<Longrightarrow> wellformed_trace t"
+  by (induction s n t rule: pre_inv_trace_assms.induct) auto
 
 lemma inv_trace_assms_Nil[simp]:
   "inv_trace_assms s [] \<longleftrightarrow> accessed_caps_invariant s"
   by (auto simp: inv_trace_assms_def)
 
-lemma inv_trace_assms_iff:
-  "inv_trace_assms s t \<longleftrightarrow> pre_inv_trace_assms s t \<and> accessed_caps_invariant (run s t)"
-  unfolding inv_trace_assms_def pre_inv_trace_assms_def
-  by (cases t rule: rev_exhaust) (auto simp: accessed_caps_trace_invariant_append_iff)
+lemma inv_trace_assms_Cons[simp]:
+  "inv_trace_assms s (e # t) \<longleftrightarrow>
+   accessed_caps_invariant s \<and> ev_assms s e \<and> wellformed_ev e \<and> inv_trace_assms (axiom_step s e) t"
+  by (auto simp: inv_trace_assms_def)
+
+lemma inv_trace_assms_take_iff_pre_inv_trace_assms:
+  assumes "n \<le> length t" and "wellformed_trace (drop n t)"
+  shows "inv_trace_assms s (take n t) \<longleftrightarrow> pre_inv_trace_assms s n t \<and> accessed_caps_invariant (run s (take n t))"
+  using assms
+  by (induction s n t rule: pre_inv_trace_assms.induct) auto
+
+lemmas inv_trace_assms_iff_pre_inv_trace_assms =
+  inv_trace_assms_take_iff_pre_inv_trace_assms[where n = "length t" and t = t for t, simplified]
 
 lemma inv_trace_assms_append_iff[simp]:
   "inv_trace_assms s (t @ t') \<longleftrightarrow> inv_trace_assms s t \<and> inv_trace_assms (run s t) t'"
-  by (auto simp: inv_trace_assms_iff pre_inv_trace_assms_append_iff)
+  by (auto simp: inv_trace_assms_def accessed_caps_trace_invariant_append_iff)
 
 lemma pre_inv_trace_assms_append_cases:
-  assumes "pre_inv_trace_assms s (t @ t')"
-  obtains (Left) "pre_inv_trace_assms s t" and "t' = []"
-  | (Bind) "inv_trace_assms s t" and "pre_inv_trace_assms (run s t) t'"
+  assumes "pre_inv_trace_assms s n (t @ t')"
+  obtains (Left) "pre_inv_trace_assms s n t" and "n \<le> length t"
+  | (Bind) "inv_trace_assms s t" and "pre_inv_trace_assms (run s t) (n - length t) t'" and "n > length t"
   using assms
-  by (cases t')
-     (auto simp: pre_inv_trace_assms_append_iff pre_inv_trace_assms_Cons inv_trace_assms_iff)
+  by (auto simp: pre_inv_trace_assms_append_iff inv_trace_assms_iff_pre_inv_trace_assms min_def split: if_splits)
+
+lemma available_caps_invariant_Zero[simp]:
+  "available_caps_invariant use_mem_caps t 0 \<longleftrightarrow> True"
+  by (auto simp: available_caps_invariant_def)
+
+lemma available_caps_invariant_Suc[simp]:
+  "available_caps_invariant use_mem_caps t (Suc n) \<longleftrightarrow>
+   available_caps_invariant use_mem_caps t n \<and> accessed_caps_invariant (run initial (take n t))"
+  by (auto simp: available_caps_invariant_def accessed_caps_invariant_def less_Suc_eq)
+
+lemma available_caps_invariant_iff_accessed_caps_trace_invariant:
+  "available_caps_invariant use_mem_caps t n \<longleftrightarrow> (n > 0 \<longrightarrow> accessed_caps_trace_invariant initial (take (n - 1) t))"
+  by (induction n)
+     (auto simp: accessed_caps_trace_invariant_def min_absorb1 dest: le_eq_less_or_eq[THEN iffD1])
 
 lemma pre_inv_trace_assms_initialI:
   assumes "available_caps_invariant use_mem_caps t n" and "trace_assms initial (take n t)"
+    and "wellformed_trace t"
     and "n \<le> length t"
     and "n = 0 \<longrightarrow> (\<forall>c \<in> initial_caps. is_tagged_method CC c \<longrightarrow> cap_invariant c)"
-  shows "pre_inv_trace_assms initial (take n t)"
-    using assms
-    unfolding available_caps_invariant_def pre_inv_trace_assms_def accessed_caps_trace_invariant_def accessed_caps_invariant_def
-    by (cases n) (auto simp: min_absorb1 butlast_take less_Suc_eq_le accessed_caps_def)
+  shows "pre_inv_trace_assms initial n t"
+  using assms
+  by (auto simp: pre_inv_trace_assms_iff available_caps_invariant_iff_accessed_caps_trace_invariant)
 
 lemma accessed_caps_trace_invariant_take:
   assumes "accessed_caps_trace_invariant s t"
@@ -1458,28 +1507,22 @@ lemma accessed_caps_trace_invariant_take:
   using assms
   by (auto simp: accessed_caps_trace_invariant_def)
 
-lemma pre_inv_trace_assms_accessed_caps_invariant:
-  assumes "pre_inv_trace_assms s t"
-  shows "accessed_caps_invariant s"
-  using assms
-  unfolding pre_inv_trace_assms_def accessed_caps_trace_invariant_def
-  by (elim conjE allE[where x = 0]) auto
-
 lemma inv_trace_assms_accessed_caps_invariant:
   assumes "inv_trace_assms s t"
   shows "accessed_caps_invariant s" and "accessed_caps_invariant (run s t)"
   using assms
-  by (auto simp: inv_trace_assms_iff intro: pre_inv_trace_assms_accessed_caps_invariant)
+  by (cases t; auto simp: inv_trace_assms_iff_pre_inv_trace_assms intro: pre_inv_trace_assms_accessed_caps_invariant)+
 
-definition "isException m \<equiv> ((\<exists>e. m = Exception e) \<or> (\<exists>msg. m = Fail msg)) \<and> ex_traces"
+definition "finished_exception m \<equiv> (\<exists>e. m = Exception e \<and> (is_isa_exception e \<longrightarrow> ex_traces))"
 
-definition finished :: "('regval,'a,'ex) monad \<Rightarrow> bool" where
-  "finished m = ((\<exists>a. m = Done a) \<or> isException m)"
+definition finished :: "('regval,'a,'e) monad \<Rightarrow> bool" where
+  "finished m = ((\<exists>a. m = Done a) \<or> (\<exists>msg. m = Fail msg) \<or> finished_exception m)"
 
 lemma finishedE:
   assumes "finished m"
   obtains (Done) a where "m = Done a"
-  | (Ex) "isException m"
+  | (Fail) msg where "m = Fail msg"
+  | (Ex) "finished_exception m"
   using assms
   by (auto simp: finished_def)
 
@@ -1487,62 +1530,62 @@ lemma finished_cases:
   assumes "finished m"
   obtains (Done) a where "m = Done a" | (Fail) msg where "m = Fail msg" | (Ex) e where "m = Exception e"
   using assms
-  by (auto simp: finished_def isException_def)
+  by (auto simp: finished_def finished_exception_def)
 
 lemma finished_Done[intro, simp]:
   "finished (Done a)"
   by (auto simp: finished_def)
 
 lemma finished_Fail[intro, simp]:
-  "finished (Fail msg) \<Longrightarrow> finished (Fail msg')"
-  unfolding finished_def isException_def
+  "finished (Fail msg')"
+  unfolding finished_def
   by auto
 
-lemma finished_Exception[intro, simp]:
-  "finished (Exception e) \<Longrightarrow> finished (Exception e')"
-  unfolding finished_def isException_def
-  by auto
-
-lemma finished_isException[intro, simp]:
-  "isException m \<Longrightarrow> finished m"
+lemma finished_exception_finished[intro, simp]:
+  "finished_exception m \<Longrightarrow> finished m"
   by (auto simp: finished_def)
 
 lemma finished_bind_left:
   assumes "finished (m \<bind> f)"
   shows "finished m"
   using assms
-  unfolding finished_def isException_def
+  unfolding finished_def finished_exception_def
   by (cases m) auto
 
 definition
   "traces_enabled m s \<equiv>
      (\<forall>t m'. (m, t, m') \<in> Traces \<and> finished m' \<longrightarrow>
-      (\<forall>n \<le> length t. pre_inv_trace_assms s (take n t) \<longrightarrow> trace_enabled s (take n t)))"
+      (\<forall>n \<le> length t. pre_inv_trace_assms s n t \<longrightarrow> trace_enabled s (take n t)))"
+
+definition "trace_raises_isa_exception t m \<equiv> (\<exists>e. runTrace t m = Some (Exception e) \<and> is_isa_exception e)"
 
 lemma traces_enabled_accepts_from_takeI:
-  assumes "hasTrace t m" and "traces_enabled m s" and "hasException t m \<or> hasFailure t m \<longrightarrow> ex_traces"
-    and "pre_inv_trace_assms s (take n t)" and "n \<le> length t"
+  assumes "hasTrace t m" and "traces_enabled m s"
+    and "trace_raises_isa_exception t m \<longrightarrow> ex_traces"
+    and "pre_inv_trace_assms s n t" and "n \<le> length t"
   shows "accepts_from s (take n t)"
   using assms
-  unfolding traces_enabled_def finished_def isException_def
-  unfolding hasTrace_iff_Traces_final hasException_iff_Traces_Exception hasFailure_iff_Traces_Fail
+  unfolding traces_enabled_def finished_def finished_exception_def
+  unfolding hasTrace_iff_Traces_final trace_raises_isa_exception_def
   unfolding runTrace_iff_Traces[symmetric]
   by (intro trace_enabled_acceptI) (auto elim!: final_cases)
 
 lemma traces_enabled_accepts_fromI:
-  assumes "hasTrace t m" and "traces_enabled m s" and "hasException t m \<or> hasFailure t m \<longrightarrow> ex_traces"
-    and "pre_inv_trace_assms s t"
+  assumes "hasTrace t m" and "traces_enabled m s"
+    and "trace_raises_isa_exception t m \<longrightarrow> ex_traces"
+    and "pre_inv_trace_assms s (length t) t"
   shows "accepts_from s t"
   using assms traces_enabled_accepts_from_takeI[OF assms(1-3), where n = "length t"]
   by auto
 
 lemma traces_enabled_acceptsI:
-  assumes "hasTrace t m" and "traces_enabled m initial" and "hasException t m \<or> hasFailure t m \<longrightarrow> ex_traces"
+  assumes "hasTrace t m" and "traces_enabled m initial"
+    and "trace_raises_isa_exception t m \<longrightarrow> ex_traces"
     and "available_caps_invariant use_mem_caps t n" and "trace_assms initial (take n t)" and "n \<le> length t"
+    and "wellformed_trace t"
   shows "accepts (take n t)"
   using assms
-  by (cases n)
-     (auto intro: traces_enabled_accepts_from_takeI traces_enabled_accepts_fromI pre_inv_trace_assms_initialI)
+  by (cases n; fastforce intro: traces_enabled_accepts_from_takeI pre_inv_trace_assms_initialI)
 
 text \<open>@{term traces_enabled} only provides guarantees if the starting state satisfies the
  capability invariants.\<close>
@@ -1550,8 +1593,8 @@ text \<open>@{term traces_enabled} only provides guarantees if the starting stat
 lemma not_accessed_caps_invariant_traces_enabled:
   assumes "\<not>accessed_caps_invariant s"
   shows "traces_enabled m s"
-  using assms pre_inv_trace_assms_accessed_caps_invariant
-  by (auto simp: traces_enabled_def)
+  using assms
+  by (auto simp: traces_enabled_def dest: pre_inv_trace_assms_accessed_caps_invariant_or_zero)
 
 named_theorems traces_enabledI
 
@@ -1562,7 +1605,7 @@ lemma traces_enabled_bind[traces_enabledI]:
 proof (unfold traces_enabled_def, intro allI impI, (elim conjE)?)
   fix t m' n
   assume t: "(m \<bind> f, t, m') \<in> Traces" and m': "finished m'" and n: "n \<le> length t"
-    and trace_assms: "pre_inv_trace_assms s (take n t)"
+    and trace_assms: "pre_inv_trace_assms s n t"
   from t show "trace_enabled s (take n t)"
   proof (cases rule: bind_Traces_cases)
     case (Left m'')
@@ -1576,17 +1619,17 @@ proof (unfold traces_enabled_def, intro allI impI, (elim conjE)?)
       case True
       then show ?thesis
         using m m' n trace_assms Bind
-        by (auto simp: traces_enabled_def dest!: finished_bind_left)
+        by (auto simp: traces_enabled_def pre_inv_trace_assms_append_iff min_absorb1 dest!: finished_bind_left)
     next
       case False
       have "trace_enabled s (take n tm)"
         using m m' n trace_assms Bind False
         unfolding traces_enabled_def
-        by (auto simp: pre_inv_trace_assms_append_iff elim!: allE[where x = tm] allE[where x = "length tm"])
+        by (auto simp: pre_inv_trace_assms_append_iff min_absorb2 elim!: allE[where x = tm] allE[where x = "length tm"])
       moreover have "trace_enabled (run s (take n tm)) (take (n - length tm) tf)"
         using f[of tm am] m' n trace_assms Bind False
         unfolding traces_enabled_def
-        by (fastforce simp: pre_inv_trace_assms_append_iff inv_trace_assms_iff)
+        by (auto simp: pre_inv_trace_assms_append_iff inv_trace_assms_iff_pre_inv_trace_assms min_absorb2)
       ultimately show ?thesis
         using Bind
         by (auto simp: trace_enabled_append_iff)
@@ -1619,20 +1662,38 @@ lemma non_cap_exp_traces_enabledI:
 proof (unfold traces_enabled_def, intro allI impI, elim conjE)
   fix t m' n
   assume "(m, t, m') \<in> Traces" and "finished m'"
-    and "pre_inv_trace_assms s (take n t)" and "n \<le> length t"
+    and "pre_inv_trace_assms s n t" and "n \<le> length t"
   then show "trace_enabled s (take n t)"
     using assms
     by (elim Traces_appendE[where t = "take n t" and t' = "drop n t", simplified])
        (auto intro: non_cap_exp_trace_enabledI)
 qed
 
-lemma exp_fails_traces_enabled:
-  assumes "exp_fails m"
+definition "exp_ends_with m P \<equiv> (\<forall>t m'. (m, t, m') \<in> Traces \<and> finished m' \<and> wellformed_trace t \<longrightarrow> P m')"
+abbreviation "exp_raises_isa_ex m \<equiv> exp_ends_with m (\<lambda>m'. \<exists>e. m' = Exception e \<and> is_isa_exception e)"
+abbreviation "exp_succeeds m \<equiv> exp_ends_with m (\<lambda>m'. \<exists>a. m' = Done a)"
+
+lemma exp_raises_ex_traces_enabled:
+  assumes "exp_raises_isa_ex m"
     and "ex_traces \<longrightarrow> traces_enabled m s"
   shows "traces_enabled m s"
+  using assms pre_inv_trace_assms_wellformed_trace
+  unfolding traces_enabled_def exp_ends_with_def finished_def finished_exception_def
+  by fastforce
+
+lemma finish_bind_cases:
+  assumes "finished (m \<bind> f)"
+  obtains (Done) a where "m = Done a" and "finished (f a)"
+  | (Fail) msg where "m = Fail msg"
+  | (Ex) e where "m = Exception e" and "finished_exception m"
+  by (rule assms[THEN finished_bind_left, THEN finishedE])
+     (use assms in \<open>auto simp: finished_exception_def\<close>)
+
+lemma exp_raises_isa_ex_bind:
+  assumes "exp_succeeds m" and "\<And>t a. Run m t a \<Longrightarrow> wellformed_trace t \<Longrightarrow> exp_raises_isa_ex (f a)"
+  shows "exp_raises_isa_ex (m \<bind> f)"
   using assms
-  unfolding traces_enabled_def finished_def isException_def
-  by blast
+  by (fastforce simp: exp_ends_with_def elim!: bind_Traces_cases finish_bind_cases)
 
 lemma traces_enabled_let[traces_enabledI]:
   assumes "traces_enabled (f y) s"
@@ -1696,7 +1757,7 @@ proof (use assms in \<open>induction "from" to step arbitrary: vars s rule: inde
     show "traces_enabled (body from vars) s"
       using body[of "from" vars "[]"] Inv_base[OF that]
       by (cases "accessed_caps_invariant s")
-         (auto simp: inv_trace_assms_iff intro: not_accessed_caps_invariant_traces_enabled)
+         (auto simp: inv_trace_assms_iff_pre_inv_trace_assms intro: not_accessed_caps_invariant_traces_enabled)
   next
     fix t vars'
     assume t: "Run (body from vars) t vars'" "inv_trace_assms s t"
@@ -1999,107 +2060,101 @@ lemma traces_enabled_try_catch:
   assumes "traces_enabled m s"
     and "\<And>tm e th m' n.
            \<lbrakk>(m, tm, Exception e) \<in> Traces; (h e, th, m') \<in> Traces; finished m'; n \<le> length (tm @ th);
-            pre_inv_trace_assms s (take n tm);
-            take (n - length tm) th = [] \<or> pre_inv_trace_assms (run s (take n tm)) (take (n - length tm) th)\<rbrakk> \<Longrightarrow>
+            pre_inv_trace_assms s n (tm @ th)\<rbrakk> \<Longrightarrow>
            trace_enabled s (take n (tm @ th))"
   shows "traces_enabled (try_catch m h) s"
 proof -
-  have *: "finished (try_catch m h) \<longleftrightarrow> (\<exists>a. m = Done a) \<or> (\<exists>msg. m = Fail msg \<and> finished m) \<or> (\<exists>e. m = Exception e \<and> (h e, [], h e) \<in> Traces \<and> finished (h e))" for m
-    by (cases m) (auto simp: finished_def isException_def)
+  have *: "finished (try_catch m h) \<longleftrightarrow> (\<exists>a. m = Done a) \<or> (\<exists>msg. m = Fail msg) \<or> (\<exists>e. m = Exception e \<and> (h e, [], h e) \<in> Traces \<and> finished (h e))" for m
+    by (cases m) (auto simp: finished_def finished_exception_def)
   show ?thesis
     using assms
     unfolding traces_enabled_def
-    by (fastforce simp: trace_enabled_append_iff pre_inv_trace_assms_append_iff *
-                  elim!: try_catch_Traces_cases)
+    by (fastforce simp: trace_enabled_append_iff * elim!: try_catch_Traces_cases)
 qed
 
-lemma traces_enabled_liftR[traces_enabledI]:
-  assumes "traces_enabled m s"
-  shows "traces_enabled (liftR m) s"
-  using assms
-  unfolding liftR_def
-  by (intro traces_enabled_try_catch) (auto simp: traces_enabled_def)
-
-lemmas traces_enabled_catch_early_return_binds[traces_enabledI] =
-  catch_early_return_bind_substs[where P = "\<lambda>m. traces_enabled m s" for s]
-
+definition "finished_early_returns m \<equiv> ((\<exists>a. m = Done a) \<or> (\<exists>a. m = Exception (Inl a)) \<or> (\<exists>msg. m = Fail msg) \<or> (\<exists>e. m = Exception (Inr e) \<and> (is_isa_exception e \<longrightarrow> ex_traces)))"
 definition
   "early_returns_enabled m s \<equiv>
-     traces_enabled m s \<and>
-     (\<forall>t a. (m, t, Exception (Inl a)) \<in> Traces \<longrightarrow>
-       (\<forall>n \<le> length t. pre_inv_trace_assms s (take n t) \<longrightarrow> trace_enabled s (take n t)))"
+     (\<forall>t m'. (m, t, m') \<in> Traces \<and> finished_early_returns m' \<longrightarrow>
+       (\<forall>n \<le> length t. pre_inv_trace_assms s n t \<longrightarrow> trace_enabled s (take n t)))"
 
-lemma traces_enabled_catch_early_return[traces_enabledI]:
-  assumes "early_returns_enabled m s"
-  shows "traces_enabled (catch_early_return m) s"
+lemma finished_early_returns_try_catch_cases:
+  assumes "finished_early_returns (try_catch m h)"
+  obtains (Done) a where "m = Done a"
+  | (Fail) msg where "m = Fail msg"
+  | (Ex) e where "m = Exception e" and "finished_early_returns (h e)"
   using assms
-  unfolding catch_early_return_def
-  by (intro traces_enabled_try_catch)
-     (auto simp: traces_enabled_def early_returns_enabled_def split: sum.splits)
+  by (cases m) (auto simp: finished_early_returns_def)
 
-lemma liftR_no_early_return[simp]:
-  shows "(liftR m, t, Exception (Inl e)) \<in> Traces \<longleftrightarrow> False"
-  by (induction m arbitrary: t) (auto simp: liftR_def elim: Traces_cases)
+lemma finished_early_returns_Inr_iff[iff]:
+  "finished_early_returns (Exception (Inr e)) \<longleftrightarrow> finished (Exception e)"
+  by (auto simp: finished_early_returns_def finished_def finished_exception_def)
+
+lemma finished_early_returnsI:
+  "finished_early_returns (Done a)"
+  "finished_early_returns (Fail msg)"
+  "finished_early_returns (Exception (Inl a))"
+  by (auto simp: finished_def finished_early_returns_def finished_exception_def)
 
 lemma early_returns_enabled_liftR[traces_enabledI]:
   assumes "traces_enabled m s"
   shows "early_returns_enabled (liftR m) s"
   using assms
-  by (auto simp: early_returns_enabled_def intro: traces_enabled_liftR)
+  unfolding liftR_def traces_enabled_def early_returns_enabled_def
+  by (fastforce elim!: try_catch_Traces_cases finished_early_returns_try_catch_cases simp: throw_def)
+
+lemma finished_try_catch_cases:
+  assumes "finished (try_catch m h)"
+  obtains (Done) a where "m = Done a"
+  | (Fail) msg where "m = Fail msg"
+  | (Ex) e where "m = Exception e" and "finished (h e)"
+  using assms
+  by (cases m) (auto simp: finished_def finished_exception_def)
+
+lemma liftR_no_early_return[simp]:
+  shows "(liftR m, t, Exception (Inl e)) \<in> Traces \<longleftrightarrow> False"
+  by (induction m arbitrary: t) (auto simp: liftR_def elim: Traces_cases)
 
 lemma early_returns_enabled_return[traces_enabledI]:
   "early_returns_enabled (return a) s"
   by (auto simp: early_returns_enabled_def traces_enabled_def)
 
-lemma early_returns_enabled_bind[traces_enabledI]:
+lemmas traces_enabled_catch_early_return_binds[traces_enabledI] =
+  catch_early_return_bind_substs[where P = "\<lambda>m. traces_enabled m s" for s]
+
+lemma early_returns_enabled_bind:
   assumes m: "early_returns_enabled m s"
     and f: "\<And>t a. Run m t a \<Longrightarrow> inv_trace_assms s t \<Longrightarrow> early_returns_enabled (f a) (run s t)"
   shows "early_returns_enabled (m \<bind> f) s"
-proof -
-  { fix t a n
-    assume "(m \<bind> f, t, Exception (Inl a)) \<in> Traces" and t: "pre_inv_trace_assms s (take n t)"
-      and n: "n \<le> length t"
-    then have "trace_enabled s (take n t)"
-    proof (cases rule: bind_Traces_cases)
-      case (Left m'')
-      then consider "m'' = Exception (Inl a)" | a' where "m'' = Done a'" and "f a' = Exception (Inl a)"
-        by (cases m'') auto
-      then show ?thesis
-        using Left m t n
-        by cases (auto simp: early_returns_enabled_def traces_enabled_def)
-    next
-      case (Bind tm am tf)
-      show ?thesis
-      proof cases
-        assume "n \<le> length tm"
-        then show ?thesis
-          using Bind m t
-          by (auto simp: trace_enabled_append_iff early_returns_enabled_def traces_enabled_def)
-      next
-        assume n': "\<not>n \<le> length tm"
-        then have "trace_enabled s (take n tm)"
-          using Bind m t
-          unfolding early_returns_enabled_def traces_enabled_def
-          by (elim conjE allE[where x = tm] allE[where x = "Done am"] allE[where x = "length tm"] impE)
-             (auto simp: pre_inv_trace_assms_append_iff)
-        moreover have "trace_enabled (run s (take n tm)) (take (n - length tm) tf)"
-          using Bind f[of tm am] t n n'
-          unfolding early_returns_enabled_def
-          by (fastforce simp: pre_inv_trace_assms_append_iff inv_trace_assms_iff)
-        ultimately show ?thesis
-          using Bind
-          by (auto simp: trace_enabled_append_iff)
-      qed
-    qed
-  }
-  then show ?thesis
-    using assms
-    by (auto intro!: traces_enabled_bind simp: early_returns_enabled_def)
+proof (unfold early_returns_enabled_def, intro allI impI, (elim conjE)?)
+  fix t m' n
+  assume "(m \<bind> f, t, m') \<in> Traces" and assms: "pre_inv_trace_assms s n t" and n: "n \<le> length t"
+    and m': "finished_early_returns m'"
+  then show "trace_enabled s (take n t)"
+  proof (cases rule: bind_Traces_cases)
+    case (Left m'')
+    then show ?thesis
+      using m m' assms n
+      by (cases m''; fastforce simp: early_returns_enabled_def finished_early_returns_def)
+  next
+    case (Bind tm am tf)
+    then show ?thesis
+      using m f[of tm am] m' assms n
+      unfolding early_returns_enabled_def
+      by (fastforce simp: trace_enabled_append_iff inv_trace_assms_iff_pre_inv_trace_assms pre_inv_trace_assms_append_iff min_def
+                    intro: finished_early_returnsI split: if_splits)
+  qed
 qed
 
 lemma early_returns_enabled_early_return[traces_enabledI]:
   "early_returns_enabled (early_return a) s"
   by (auto simp: early_returns_enabled_def early_return_def throw_def traces_enabled_def)
+
+lemma traces_enabled_catch_early_return_enabled_let[traces_enabledI]:
+  assumes "traces_enabled (catch_early_return (f y)) s"
+  shows "traces_enabled (catch_early_return (let x = y in f x)) s"
+  using assms
+  by auto
 
 lemma early_returns_enabled_let[traces_enabledI]:
   assumes "early_returns_enabled (f y) s"
@@ -2130,14 +2185,16 @@ lemma early_returns_enabled_and_boolM[traces_enabledI]:
     and "\<And>t. Run m1 t True \<Longrightarrow> early_returns_enabled m2 (run s t)"
   shows "early_returns_enabled (and_boolM m1 m2) s"
   using assms
-  by (auto simp: and_boolM_def intro!: traces_enabledI intro: non_cap_exp_traces_enabledI non_cap_expI)
+  by (auto simp: and_boolM_def intro!: early_returns_enabled_bind early_returns_enabled_return
+           intro: non_cap_exp_traces_enabledI non_cap_expI)
 
 lemma early_returns_enabled_or_boolM[traces_enabledI]:
   assumes "early_returns_enabled m1 s"
     and "\<And>t. Run m1 t False \<Longrightarrow> early_returns_enabled m2 (run s t)"
   shows "early_returns_enabled (or_boolM m1 m2) s"
   using assms
-  by (auto simp: or_boolM_def intro!: traces_enabledI intro: non_cap_exp_traces_enabledI non_cap_expI)
+  by (auto simp: or_boolM_def intro!: early_returns_enabled_bind early_returns_enabled_return
+           intro: non_cap_exp_traces_enabledI non_cap_expI)
 
 lemma early_returns_enabled_foreachM_inv:
   assumes "\<And>x vars s. P vars s \<Longrightarrow> x \<in> set xs \<Longrightarrow> early_returns_enabled (body x vars) s"
@@ -2145,7 +2202,16 @@ lemma early_returns_enabled_foreachM_inv:
     and "P vars s"
   shows "early_returns_enabled (foreachM xs vars body) s"
   by (use assms in \<open>induction xs arbitrary: vars s\<close>;
-      fastforce intro!: traces_enabledI intro: non_cap_exp_traces_enabledI non_cap_expI)
+      fastforce intro!: early_returns_enabled_bind early_returns_enabled_return
+                intro: non_cap_exp_traces_enabledI non_cap_expI)
+
+lemma traces_enabled_catch_early_return:
+  assumes "early_returns_enabled m s"
+  shows "traces_enabled (catch_early_return m) s"
+  using assms
+  unfolding catch_early_return_def traces_enabled_def early_returns_enabled_def
+  by (fastforce elim!: try_catch_Traces_cases finished_try_catch_cases intro: finished_early_returnsI
+                simp: throw_def split: sum.splits)
 
 lemma non_cap_exp_Run_inv_traces_enabled_runE:
   assumes "Run m1 t a" and "non_cap_exp m1" and "traces_enabled m2 s"
@@ -2188,10 +2254,19 @@ lemmas traces_enabled_builtin_combinatorsI =
   early_returns_enabled_bind early_returns_enabled_and_boolM early_returns_enabled_or_boolM
 
 named_theorems traces_enabled_split
-declare option.split[where P = "\<lambda>m. traces_enabled m s" for s, traces_enabled_split]
-declare prod.split[where P = "\<lambda>m. traces_enabled m s" for s, traces_enabled_split]
-declare sum.split[where P = "\<lambda>m. traces_enabled m s" for s, traces_enabled_split]
-declare bool.split[where P = "\<lambda>m. traces_enabled m s" for s, traces_enabled_split]
+
+lemmas traces_enabled_split_base[traces_enabled_split] =
+  option.split[where P = "\<lambda>m. traces_enabled m s" for s]
+  prod.split[where P = "\<lambda>m. traces_enabled m s" for s]
+  sum.split[where P = "\<lambda>m. traces_enabled m s" for s]
+  bool.split[where P = "\<lambda>m. traces_enabled m s" for s]
+
+lemmas traces_enabled_catch_early_return_split_base[traces_enabled_split] =
+  if_split[where P = "\<lambda>m. traces_enabled (catch_early_return m) s" for s]
+  option.split[where P = "\<lambda>m. traces_enabled (catch_early_return m) s" for s]
+  prod.split[where P = "\<lambda>m. traces_enabled (catch_early_return m) s" for s]
+  sum.split[where P = "\<lambda>m. traces_enabled (catch_early_return m) s" for s]
+  bool.split[where P = "\<lambda>m. traces_enabled (catch_early_return m) s" for s]
 
 method traces_enabled_foreachM_intro uses assms simp =
   (match conclusion in \<open>traces_enabled (foreachM _ _ _) _\<close> \<Rightarrow>
@@ -2208,6 +2283,7 @@ method traces_enabled_step uses simp intro elim assms =
     | (rule traces_enabledI TrueI)
     | (rule traces_enabled_split[THEN iffD2]; intro allI conjI impI)
     | (traces_enabled_foreachM_intro assms: assms simp: simp)
+    | (rule traces_enabled_catch_early_return)
     | (rule insert_subset[where B="insert y C" for y C, THEN iffD2], simp(no_asm)))
 
 method traces_enabledI_with methods solve uses simp intro elim assms =
@@ -2246,14 +2322,15 @@ locale Cap_Axiom_Inv_Automaton =
     and read_non_special_regs_enabled: "\<And>r v. r \<notin> PCC ISA \<union> IDC ISA \<union> KCC ISA \<union> read_privileged_regs ISA \<Longrightarrow> enabled s (E_read_reg r v)"
 begin
 
-definition "isException m \<equiv> ((\<exists>e. m = Exception e) \<or> (\<exists>msg. m = Fail msg)) \<and> ex_traces"
+definition "isException m \<equiv> (\<exists>e. m = Exception e) \<and> ex_traces"
 
 definition finished :: "('regval,'a,'ex) monad \<Rightarrow> bool" where
-  "finished m = ((\<exists>a. m = Done a) \<or> isException m)"
+  "finished m = ((\<exists>a. m = Done a) \<or> (\<exists>msg. m = Fail msg) \<or> isException m)"
 
 lemma finishedE:
   assumes "finished m"
   obtains (Done) a where "m = Done a"
+  | (Fail) msg where "m = Fail msg"
   | (Ex) "isException m"
   using assms
   by (auto simp: finished_def)
@@ -2269,7 +2346,7 @@ lemma finished_Done[intro, simp]:
   by (auto simp: finished_def)
 
 lemma finished_Fail[intro, simp]:
-  "finished (Fail msg) \<Longrightarrow> finished (Fail msg')"
+  "finished (Fail msg')"
   unfolding finished_def isException_def
   by auto
 
@@ -2294,12 +2371,12 @@ definition
      \<forall>t m'. (m, t, m') \<in> Traces \<and> finished m' \<and> reads_regs_from inv_regs t regs \<and> invariant regs \<longrightarrow> trace_enabled s t"
 
 lemma traces_enabled_accepts_fromI:
-  assumes "hasTrace t m" and "traces_enabled m s regs" and "hasException t m \<or> hasFailure t m \<longrightarrow> ex_traces"
+  assumes "hasTrace t m" and "traces_enabled m s regs" and "hasException t m \<longrightarrow> ex_traces"
     and "reads_regs_from inv_regs t regs" and "invariant regs"
   shows "accepts_from s t"
   using assms
   unfolding traces_enabled_def finished_def isException_def
-  unfolding hasTrace_iff_Traces_final hasException_iff_Traces_Exception hasFailure_iff_Traces_Fail
+  unfolding hasTrace_iff_Traces_final hasException_iff_Traces_Exception
   unfolding runTrace_iff_Traces[symmetric]
   by (intro trace_enabled_acceptI) (auto elim!: final_cases)
 
@@ -2310,8 +2387,10 @@ lemma traces_enabled_bind[traces_enabledI]:
     and "\<And>t a. Run_inv m t a regs \<Longrightarrow> traces_enabled (f a) (run s t) (the (updates_regs inv_regs t regs))"
   shows "traces_enabled (m \<bind> f) s regs"
   using assms
-  by (auto simp: traces_enabled_def Run_inv_def regstate_simp trace_enabled_append_iff
-           dest!: finished_bind_left elim!: bind_Traces_cases elim!: runs_preserve_invariantE; fastforce)
+  apply (auto simp: traces_enabled_def Run_inv_def regstate_simp trace_enabled_append_iff
+           dest!: finished_bind_left elim!: bind_Traces_cases elim!: runs_preserve_invariantE)
+  apply blast apply fastforce
+  done
 
 lemma non_cap_trace_enabledI:
   assumes "non_cap_trace t"
@@ -2390,7 +2469,7 @@ lemma traces_enabled_try_catch:
            trace_enabled s (tm @ th)"
   shows "traces_enabled (try_catch m h) s regs"
 proof -
-  have *: "finished (try_catch m h) \<longleftrightarrow> (\<exists>a. m = Done a) \<or> (\<exists>msg. m = Fail msg \<and> finished m) \<or> (\<exists>e. m = Exception e \<and> (h e, [], h e) \<in> Traces \<and> finished (h e))" for m
+  have *: "finished (try_catch m h) \<longleftrightarrow> (\<exists>a. m = Done a) \<or> (\<exists>msg. m = Fail msg) \<or> (\<exists>e. m = Exception e \<and> (h e, [], h e) \<in> Traces \<and> finished (h e))" for m
     by (cases m) (auto simp: finished_def isException_def)
   show ?thesis
     using assms
@@ -2615,6 +2694,8 @@ locale Write_Cap_Assm_Automaton =
   and ex_traces :: bool and use_mem_caps :: bool
   and invoked_caps :: "'cap set" and invoked_indirect_caps :: "'cap set" +
   fixes ev_assms :: "('cap, 'regval) axiom_state \<Rightarrow> 'regval event \<Rightarrow> bool"
+  and is_isa_exception :: "'e \<Rightarrow> bool"
+  and wellformed_ev :: "'regval event \<Rightarrow> bool"
 begin
 
 sublocale Cap_Axiom_Assm_Automaton where enabled = enabled
@@ -2679,17 +2760,18 @@ lemma traces_enabled_write_memt[traces_enabledI]:
                \<and> mem_bytes_of_bits BCb data = Some bytes
                \<and> cap_of_mem_bytes_method CC bytes tag = Some c
                \<and> ev_assms s (E_write_memt wk addr' (nat sz) bytes tag r)
+               \<and> wellformed_ev (E_write_memt wk addr' (nat sz) bytes tag r)
              \<longrightarrow> c \<in> derivable_caps s"
   shows "traces_enabled (write_memt BCa BCb wk addr sz data tag) s"
   using assms
   unfolding write_memt_def maybe_fail_def derivable_caps_def
-  by (fastforce simp: traces_enabled_def pre_inv_trace_assms_def take_Cons
-                split: option.splits nat.splits elim: Traces_cases)
+  by (fastforce simp: traces_enabled_def take_Cons split: option.splits nat.splits elim: Traces_cases)
 
 lemma traces_enabled_reg_axioms:
   assumes "traces_enabled m initial" and "hasTrace t m"
     and "available_caps_invariant use_mem_caps t n" and "trace_assms initial (take n t)" and "n \<le> length t"
-    and "hasException t m \<or> hasFailure t m \<longrightarrow> ex_traces"
+    and "wellformed_trace t"
+    and "trace_raises_isa_exception t m \<longrightarrow> ex_traces"
   shows "store_cap_reg_axiom CC ISA ex_traces initial_caps use_mem_caps invoked_caps invoked_indirect_caps (take n t)"
     and "store_cap_mem_axiom CC ISA initial_caps use_mem_caps invoked_indirect_caps (take n t)"
     and "read_reg_axiom CC ISA ex_traces (take n t)"
@@ -2757,7 +2839,7 @@ lemma traces_enabled_write_reg:
 lemma traces_enabled_reg_axioms:
   assumes "traces_enabled m initial regs" and "hasTrace t m"
     and "reads_regs_from inv_regs t regs" and "invariant regs"
-    and "hasException t m \<or> hasFailure t m \<longrightarrow> ex_traces"
+    and "hasException t m \<longrightarrow> ex_traces"
   shows "store_cap_reg_axiom CC ISA ex_traces initial_caps use_mem_caps invoked_caps invoked_indirect_caps t"
     and "store_cap_mem_axiom CC ISA initial_caps use_mem_caps invoked_indirect_caps t"
     and "read_reg_axiom CC ISA ex_traces t"
@@ -2932,7 +3014,9 @@ locale Mem_Assm_Automaton =
     and translation_assms :: "'regval event \<Rightarrow> bool"
     and is_fetch :: bool and ex_traces :: bool and use_mem_caps :: bool
     and invoked_indirect_caps :: "'cap set" +
-  fixes ev_assms :: "('cap, 'regval) axiom_state \<Rightarrow> 'regval event \<Rightarrow> bool"
+  fixes is_isa_exception :: "'e \<Rightarrow> bool"
+    and ev_assms :: "('cap, 'regval) axiom_state \<Rightarrow> 'regval event \<Rightarrow> bool"
+    and wellformed_ev :: "'regval event \<Rightarrow> bool"
   assumes translation_assmsI: "\<And>s e. ev_assms s e \<Longrightarrow> translation_assms e"
 begin
 
@@ -2967,7 +3051,8 @@ lemma translation_assms_traceI:
 lemma traces_enabled_mem_axioms:
   assumes "traces_enabled m initial" and "hasTrace t m"
     and "available_caps_invariant use_mem_caps t n" and "trace_assms initial (take n t)" and "n \<le> length t"
-    and "hasException t m \<or> hasFailure t m \<longrightarrow> ex_traces"
+    and "wellformed_trace t"
+    and "trace_raises_isa_exception t m \<longrightarrow> ex_traces"
   shows "store_mem_axiom CC ISA initial_caps use_mem_caps invoked_indirect_caps (take n t)"
     and "store_tag_axiom CC ISA (take n t)"
     and "load_mem_axiom CC ISA is_fetch initial_caps use_mem_caps invoked_indirect_caps (take n t)"
@@ -2981,7 +3066,7 @@ lemma traces_enabled_Read_mem:
     and "\<And>v. enabled s (E_read_mem rk paddr sz v)"
   shows "traces_enabled (Read_mem rk paddr sz m) s"
   using assms
-  by (fastforce simp: traces_enabled_def take_Cons pre_inv_trace_assms_Cons split: nat.splits
+  by (fastforce simp: traces_enabled_def take_Cons split: nat.splits
                 elim!: Traces_cases[where m = "Read_mem rk paddr sz m"])
 
 lemma traces_enabled_read_mem:
@@ -2997,7 +3082,7 @@ lemma traces_enabled_Read_memt:
     and "\<And>v tag. enabled s (E_read_memt rk paddr sz (v, tag))"
   shows "traces_enabled (Read_memt rk paddr sz m) s"
   using assms
-  by (fastforce simp: traces_enabled_def take_Cons pre_inv_trace_assms_Cons split: nat.splits
+  by (fastforce simp: traces_enabled_def take_Cons split: nat.splits
                 elim!: Traces_cases[where m = "Read_memt rk paddr sz m"])
 
 lemma traces_enabled_read_memt:
@@ -3049,7 +3134,7 @@ lemma non_mem_exp_traces_enabledI:
 lemma traces_enabled_mem_axioms:
   assumes "traces_enabled m initial regs" and "hasTrace t m"
     and "reads_regs_from inv_regs t regs" and "invariant regs"
-    and "hasException t m \<or> hasFailure t m \<longrightarrow> ex_traces"
+    and "hasException t m \<longrightarrow> ex_traces"
     and "translation_assms_trace t"
   shows "store_mem_axiom CC ISA initial_caps use_mem_caps invoked_indirect_caps t"
     and "store_tag_axiom CC ISA t"
